prove sexpexp_expsexp

parsing/fromSexpScript.sml
@@ -45,6 +45,13 @@ val pat_ind =
   |> SIMP_RULE list_ss []
   |> UNDISCH_ALL |> CONJUNCT1
   |> DISCH_ALL |> Q.GEN`P`
+
+val exp_ind =
+  (TypeBase.induction_of``:exp``)
+  |> Q.SPECL[`P`,`EVERY (P o SND o SND)`,`P o SND o SND`,`EVERY (P o SND)`,`P o SND`,`P o SND`,`EVERY P`]
+  |> SIMP_RULE list_ss []
+  |> UNDISCH_ALL |> CONJUNCT1
+  |> DISCH_ALL |> Q.GEN`P`
 (* -- *)
 
 
@@ -258,6 +265,50 @@ val sexppat_def = tDefine "sexppat" `
    >- metis_tac[rich_listTheory.EL_MEM, DECIDE ``0n < 1``, listTheory.EL,
                 dstrip_sexp_size])
 
+val sexpop_def = Define`
+  (sexpop (SX_SYM s) =
+  if s = "OpnPlus" then SOME (Opn Plus) else
+  if s = "OpnMinus" then SOME (Opn Minus) else
+  if s = "OpnTimes" then SOME (Opn Times) else
+  if s = "OpnDivide" then SOME (Opn Divide) else
+  if s = "OpnModulo" then SOME (Opn Modulo) else
+  if s = "OpbLt" then SOME (Opb Lt) else
+  if s = "OpbGt" then SOME (Opb Gt) else
+  if s = "OpbLeq" then SOME (Opb Leq) else
+  if s = "OpbGeq" then SOME (Opb Geq) else
+  if s = "Equality" then SOME Equality else
+  if s = "Opapp" then SOME Opapp else
+  if s = "Opassign" then SOME Opassign else
+  if s = "Opref" then SOME Opref else
+  if s = "Opderef" then SOME Opderef else
+  if s = "Aw8alloc" then SOME Aw8alloc else
+  if s = "Aw8sub" then SOME Aw8sub else
+  if s = "Aw8length" then SOME Aw8length else
+  if s = "Aw8update" then SOME Aw8update else
+  if s = "Ord" then SOME Ord else
+  if s = "Chr" then SOME Chr else
+  if s = "ChopbLt" then SOME (Chopb Lt) else
+  if s = "ChopbGt" then SOME (Chopb Gt) else
+  if s = "ChopbLeq" then SOME (Chopb Leq) else
+  if s = "ChopbGeq" then SOME (Chopb Geq) else
+  if s = "Explode" then SOME Explode else
+  if s = "Implode" then SOME Implode else
+  if s = "Strlen" then SOME Strlen else
+  if s = "VfromList" then SOME VfromList else
+  if s = "Vsub" then SOME Vsub else
+  if s = "Vlength" then SOME Vlength else
+  if s = "Aalloc" then SOME Aalloc else
+  if s = "Asub" then SOME Asub else
+  if s = "Alength" then SOME Alength else
+  if s = "Aupdate" then SOME Aupdate else NONE) ∧
+  (sexpop _ = NONE)`;
+
+val sexplop_def = Define`
+  (sexplop (SX_SYM s) =
+   if s = "And" then SOME And else
+   if s = "Or" then SOME Or else NONE) ∧
+  (sexplop _ = NONE)`;
+
 val sexpexp_def = tDefine "sexpexp" `
   sexpexp s =
     do
@@ -275,22 +326,51 @@ val sexpexp_def = tDefine "sexpexp" `
                    (sexpopt (sexpid odestSXSTR) (EL 0 args))
                    (sexplist sexpexp (EL 1 args))) ++
       guard (nm = "Var" ∧ LENGTH args = 1)
-            (lift Var (sexpid odestSXSTR (EL 0 args)))
+            (lift Var (sexpid odestSXSTR (EL 0 args))) ++
+      guard (nm = "Fun" ∧ LENGTH args = 2)
+            (lift2 Fun (odestSXSTR (EL 0 args)) (sexpexp (EL 1 args))) ++
+      guard (nm = "App" ∧ LENGTH args = 2)
+            (lift2 App (sexpop (EL 0 args)) (sexplist sexpexp (EL 1 args))) ++
+      guard (nm = "Log" ∧ LENGTH args = 3)
+            (lift Log (sexplop (EL 0 args)) <*>
+                      (sexpexp (EL 1 args)) <*>
+                      (sexpexp (EL 2 args))) ++
+      guard (nm = "If" ∧ LENGTH args = 3)
+            (lift If (sexpexp (EL 0 args)) <*>
+                     (sexpexp (EL 1 args)) <*>
+                     (sexpexp (EL 2 args))) ++
+      guard (nm = "Mat" ∧ LENGTH args = 2)
+            (lift2 Mat
+              (sexpexp (EL 0 args))
+              (sexplist (sexppair sexppat sexpexp) (EL 1 args))) ++
+      guard (nm = "Let" ∧ LENGTH args = 3)
+            (lift Let (sexpopt odestSXSTR (EL 0 args)) <*>
+                      (sexpexp (EL 1 args)) <*>
+                      (sexpexp (EL 2 args))) ++
+      guard (nm = "Letrec" ∧ LENGTH args = 2)
+            (lift2 Letrec
+              (sexplist (sexppair odestSXSTR (sexppair odestSXSTR sexpexp)) (EL 0 args))
+              (sexpexp (EL 1 args)))
     od
 `
   (WF_REL_TAC `measure sexp_size` >> simp[] >> rpt strip_tac
-   >- (qcase_tac `sxMEM sx0 (EL 1 args)` >>
+   >> TRY
+     (qcase_tac `sxMEM sx0 (EL 1 args)` >>
        `sexp_size sx0 < sexp_size (EL 1 args)` by simp[sxMEM_sizelt] >>
        rw[] >> fs[sexp_size_def] >>
        `sexp_size (EL 1 args) < sexp_size s`
          by simp[dstrip_sexp_size, rich_listTheory.EL_MEM] >>
        simp[])
-   >- metis_tac[rich_listTheory.EL_MEM, listTheory.EL, DECIDE ``1n < 2``,
-                dstrip_sexp_size, sxMEM_sizelt, arithmeticTheory.LESS_TRANS]
-   >- metis_tac[rich_listTheory.EL_MEM, listTheory.EL, DECIDE ``0n < 2``,
-                dstrip_sexp_size]
-   >- metis_tac[rich_listTheory.EL_MEM, listTheory.EL, DECIDE ``0n < 1``,
-                dstrip_sexp_size])
+   >- (
+     rw[] >>
+     imp_res_tac dstrip_sexp_size >>
+     imp_res_tac sxMEM_sizelt >>
+     fs[sexp_size_def] >>
+     `sexp_size a < sexp_size (HD args)` by decide_tac >>
+     metis_tac[listTheory.EL,rich_listTheory.EL_MEM,DECIDE``0n < 2``,arithmeticTheory.LESS_TRANS])
+   >> metis_tac[rich_listTheory.EL_MEM, listTheory.EL,
+                DECIDE ``1n < 2 ∧ 0n < 2 ∧ 0n < 1 ∧ 2n < 3 ∧ 0n < 3 ∧ 1n < 3``,
+                dstrip_sexp_size, sxMEM_sizelt, arithmeticTheory.LESS_TRANS])
 
 val sexptype_def_def = Define`
   sexptype_def =
@@ -451,7 +531,7 @@ val opsexp_def = Define`
   (opsexp (Chopb Lt) = SX_SYM "ChopbLt") ∧
   (opsexp (Chopb Gt) = SX_SYM "ChopbGt") ∧
   (opsexp (Chopb Leq)= SX_SYM "ChopbLeq") ∧
-  (opsexp (Chopb Geq)= SX_SYM "ChopbLeq") ∧
+  (opsexp (Chopb Geq)= SX_SYM "ChopbGeq") ∧
   (opsexp Explode = SX_SYM "Explode") ∧
   (opsexp Implode = SX_SYM "Implode") ∧
   (opsexp Strlen = SX_SYM "Strlen") ∧
@@ -663,9 +743,26 @@ val sexppat_patsexp = Q.store_thm("sexppat_patsexp[simp]",
     fs[listTheory.EVERY_MEM] >> metis_tac[]) >>
   rw[] >> simp[patsexp_def,Once sexppat_def]);
 
+val sexpop_opsexp = Q.store_thm("sexpop_opsexp[simp]",
+  `sexpop (opsexp op) = SOME op`,
+  Cases_on`op`>>rw[sexpop_def,opsexp_def]>>
+  Cases_on`o'`>>rw[sexpop_def,opsexp_def]);
+
+val sexplop_lopsexp = Q.store_thm("sexplop_lopsexp[simp]",
+  `sexplop (lopsexp l) = SOME l`,
+  Cases_on`l`>>EVAL_TAC)
+
 val sexpexp_expsexp = Q.store_thm("sexpexp_expsexp[simp]",
   `sexpexp (expsexp e) = SOME e`,
-  cheat)
+  qid_spec_tac`e` >>
+  ho_match_mp_tac exp_ind >> rw[] >>
+  rw[expsexp_def] >> rw[Once sexpexp_def] >>
+  match_mp_tac sexplist_listsexp_matchable >>
+  exists_g_tac >> simp[] >>
+  fs[listTheory.EVERY_MEM] >>
+  qx_gen_tac`p`>>PairCases_on`p` >> simp[] >>
+  simp[sexppair_def] >>
+  rw[] >> res_tac >> fs[]);
 
 val sexpdec_decsexp = Q.store_thm("sexpdec_decsexp[simp]",
   `sexpdec (decsexp d) = SOME d`,
